src/invariant/InvariantBase.v
@@ -1,0 +1,238 @@
+Require Import Omega.
+Require Import RelationClasses.
+
+Require Import sflib.
+Require Import paco.
+
+Require Import Axioms.
+Require Import Basic.
+Require Import DataStructure.
+Require Import DenseOrder.
+Require Import Event.
+Require Import Time.
+Require Import Language.
+Require Import View.
+Require Import Cell.
+Require Import Memory.
+Require Import Commit.
+Require Import Thread.
+Require Import Configuration.
+
+Require Import PromiseConsistent.
+Require Import ReorderThreadStepSame.
+
+Set Implicit Arguments.
+
+
+Inductive step_evt lang (e1 e2:Thread.t lang): Prop :=
+| step_evt_intro
+    e
+    (STEP: Thread.step e e1 e2)
+.
+
+Inductive program_step_evt lang (e1 e2:Thread.t lang): Prop :=
+| program_step_evt_intro
+    e
+    (STEP: Thread.program_step e e1 e2)
+.
+
+Inductive promise_step_evt lang (e1 e2:Thread.t lang): Prop :=
+| promise_step_evt_intro
+    e
+    (STEP: Thread.promise_step e e1 e2)
+.
+
+Lemma step_evt_future lang (e1 e2:Thread.t lang)
+      (STEP: step_evt e1 e2)
+      (WF1: Local.wf e1.(Thread.local) e1.(Thread.memory))
+      (SC1: Memory.closed_timemap e1.(Thread.sc) e1.(Thread.memory))
+      (CLOSED1: Memory.closed e1.(Thread.memory)):
+  <<WF2: Local.wf e2.(Thread.local) e2.(Thread.memory)>> /\
+  <<SC2: Memory.closed_timemap e2.(Thread.sc) e2.(Thread.memory)>> /\
+  <<CLOSED2: Memory.closed e2.(Thread.memory)>> /\
+  <<COMMIT_FUTURE: Commit.le e1.(Thread.local).(Local.commit) e2.(Thread.local).(Local.commit)>> /\
+  <<SC_FUTURE: TimeMap.le e1.(Thread.sc) e2.(Thread.sc)>> /\
+  <<MEM_FUTURE: Memory.future e1.(Thread.memory) e2.(Thread.memory)>>.
+Proof.
+  inv STEP. eapply Thread.step_future; eauto.
+Qed.
+
+Lemma rtc_step_evt_future lang (e1 e2:Thread.t lang)
+      (STEP: rtc (@step_evt lang) e1 e2)
+      (WF1: Local.wf e1.(Thread.local) e1.(Thread.memory))
+      (SC1: Memory.closed_timemap e1.(Thread.sc) e1.(Thread.memory))
+      (CLOSED1: Memory.closed e1.(Thread.memory)):
+  <<WF2: Local.wf e2.(Thread.local) e2.(Thread.memory)>> /\
+  <<SC2: Memory.closed_timemap e2.(Thread.sc) e2.(Thread.memory)>> /\
+  <<CLOSED2: Memory.closed e2.(Thread.memory)>> /\
+  <<COMMIT_FUTURE: Commit.le e1.(Thread.local).(Local.commit) e2.(Thread.local).(Local.commit)>> /\
+  <<SC_FUTURE: TimeMap.le e1.(Thread.sc) e2.(Thread.sc)>> /\
+  <<MEM_FUTURE: Memory.future e1.(Thread.memory) e2.(Thread.memory)>>.
+Proof.
+  revert WF1. induction STEP.
+  - i. splits; ss; refl.
+  - i. exploit step_evt_future; eauto. i. des.
+    exploit IHSTEP; eauto. i. des.
+    splits; ss; etrans; eauto.
+Qed.
+
+Lemma promise_step_evt_future lang (e1 e2:Thread.t lang)
+      (STEP: promise_step_evt e1 e2)
+      (WF1: Local.wf e1.(Thread.local) e1.(Thread.memory))
+      (SC1: Memory.closed_timemap e1.(Thread.sc) e1.(Thread.memory))
+      (CLOSED1: Memory.closed e1.(Thread.memory)):
+  <<WF2: Local.wf e2.(Thread.local) e2.(Thread.memory)>> /\
+  <<SC2: Memory.closed_timemap e2.(Thread.sc) e2.(Thread.memory)>> /\
+  <<CLOSED2: Memory.closed e2.(Thread.memory)>> /\
+  <<COMMIT_FUTURE: Commit.le e1.(Thread.local).(Local.commit) e2.(Thread.local).(Local.commit)>> /\
+  <<SC_FUTURE: TimeMap.le e1.(Thread.sc) e2.(Thread.sc)>> /\
+  <<MEM_FUTURE: Memory.future e1.(Thread.memory) e2.(Thread.memory)>> /\
+  <<STATE: e1.(Thread.state) = e2.(Thread.state)>>.
+Proof.
+  inv STEP. exploit Thread.promise_step_future; eauto. i. des.
+  inv STEP0. ss. esplits; eauto. refl.
+Qed.
+
+Lemma rtc_promise_step_evt_future lang (e1 e2:Thread.t lang)
+      (STEP: rtc (@promise_step_evt lang) e1 e2)
+      (WF1: Local.wf e1.(Thread.local) e1.(Thread.memory))
+      (SC1: Memory.closed_timemap e1.(Thread.sc) e1.(Thread.memory))
+      (CLOSED1: Memory.closed e1.(Thread.memory)):
+  <<WF2: Local.wf e2.(Thread.local) e2.(Thread.memory)>> /\
+  <<SC2: Memory.closed_timemap e2.(Thread.sc) e2.(Thread.memory)>> /\
+  <<CLOSED2: Memory.closed e2.(Thread.memory)>> /\
+  <<COMMIT_FUTURE: Commit.le e1.(Thread.local).(Local.commit) e2.(Thread.local).(Local.commit)>> /\
+  <<SC_FUTURE: TimeMap.le e1.(Thread.sc) e2.(Thread.sc)>> /\
+  <<MEM_FUTURE: Memory.future e1.(Thread.memory) e2.(Thread.memory)>> /\
+  <<STATE: e1.(Thread.state) = e2.(Thread.state)>>.
+Proof.
+  revert WF1. induction STEP.
+  - i. splits; ss; refl.
+  - i. exploit promise_step_evt_future; eauto. i. des.
+    exploit IHSTEP; eauto. i. des.
+    splits; ss; etrans; eauto.
+Qed.
+
+Lemma tau_program_step_program_step_evt:
+  SmallStep.tau_program_step <3= program_step_evt.
+Proof.
+  i. inv PR. econs. eauto.
+Qed.
+
+Lemma tau_step_step_evt:
+  Thread.tau_step <3= step_evt.
+Proof.
+  i. inv PR. econs. eauto.
+Qed.
+
+Lemma program_step_evt_step_evt:
+  program_step_evt <3= step_evt.
+Proof.
+  i. inv PR. econs. eauto.
+Qed.
+
+Lemma promise_step_evt_step_evt:
+  promise_step_evt <3= step_evt.
+Proof.
+  i. inv PR. econs. eauto.
+Qed.
+
+Lemma rtc_step_evt_promise_consistent
+      lang th1 th2
+      (STEP: rtc (@step_evt lang) th1 th2)
+      (CONS: promise_consistent th2.(Thread.local))
+      (WF1: Local.wf th1.(Thread.local) th1.(Thread.memory))
+      (SC1: Memory.closed_timemap th1.(Thread.sc) th1.(Thread.memory))
+      (MEM1: Memory.closed th1.(Thread.memory)):
+  promise_consistent th1.(Thread.local).
+Proof.
+  revert_until STEP. induction STEP; auto. i.
+  inv H. exploit Thread.step_future; eauto. i. des.
+  eapply step_promise_consistent; eauto.
+Qed.
+
+Lemma steps_pf_steps_aux
+      lang
+      n e1 e3
+      (STEPS: rtcn (@step_evt lang) n e1 e3)
+      (CONS: promise_consistent e3.(Thread.local))
+      (WF1: Local.wf e1.(Thread.local) e1.(Thread.memory))
+      (SC1: Memory.closed_timemap e1.(Thread.sc) e1.(Thread.memory))
+      (MEM1: Memory.closed e1.(Thread.memory)):
+  exists n' e2,
+    <<N: n' <= n>> /\
+    <<STEPS1: rtcn (@program_step_evt lang) n' e1 e2>> /\
+    <<STEPS2: rtc (@promise_step_evt lang) e2 e3>>.
+Proof.
+  revert_until n. induction n using strong_induction; i.
+  inv STEPS.
+  { esplits; eauto. }
+  inv A12. inv STEP; cycle 1.
+  { exploit Thread.program_step_future; eauto. i. des.
+    exploit IH; eauto. i. des.
+    esplits; cycle 1.
+    + econs 2; eauto. econs; eauto.
+    + auto.
+    + omega.
+  }
+  exploit Thread.promise_step_future; eauto. i. des.
+  exploit IH; try exact A23; try refl; eauto. i. des.
+  inv STEPS1.
+  { esplits; cycle 1.
+    - eauto.
+    - econs; eauto. econs. eauto.
+    - omega.
+  }
+  inversion A12. exploit Thread.program_step_future; eauto. i. des.
+  exploit reorder_promise_program; eauto.
+  { exploit rtcn_rtc; try exact A0; eauto. i.
+    eapply rtc_step_evt_promise_consistent; try exact CONS; eauto.
+    etrans.
+    - eapply rtc_implies; try exact x0; eauto.
+      apply program_step_evt_step_evt.
+    - eapply rtc_implies; try exact STEPS2; eauto.
+      apply promise_step_evt_step_evt.
+  }
+  i. des.
+  exploit Thread.program_step_future; eauto. i. des.
+  unguardH STEP2. des.
+  - subst. esplits; cycle 1.
+    + econs 2; eauto. econs. eauto.
+    + auto.
+    + omega.
+  - exploit Thread.promise_step_future; try exact STEP2; eauto. i. des.
+    assert (STEPS: rtcn (step_evt (lang:=lang)) (S n) th1' e2).
+    { econs 2.
+      - econs. econs 1. apply STEP2.
+      - eapply rtcn_imply; try exact A0. i. inv PR. econs; eauto.
+    }
+    exploit rtcn_rtc; eauto. i.
+    exploit rtc_step_evt_future; eauto. i. des.
+    exploit IH; try exact STEPS; eauto.
+    { omega. }
+    { eapply rtc_step_evt_promise_consistent; try exact CONS; eauto.
+      eapply rtc_implies; try exact STEPS2; eauto.
+      apply promise_step_evt_step_evt.
+    }
+    i. des. esplits; cycle 1.
+    + econs; [|eauto]. econs; eauto.
+    + etrans; eauto.
+    + omega.
+Qed.
+
+Lemma steps_pf_steps
+      lang
+      e1 e3
+      (STEPS: rtc (@step_evt lang) e1 e3)
+      (CONS: promise_consistent e3.(Thread.local))
+      (WF1: Local.wf e1.(Thread.local) e1.(Thread.memory))
+      (SC1: Memory.closed_timemap e1.(Thread.sc) e1.(Thread.memory))
+      (MEM1: Memory.closed e1.(Thread.memory)):
+  exists e2,
+    <<STEPS1: rtc (@program_step_evt lang) e1 e2>> /\
+    <<STEPS2: rtc (@promise_step_evt lang) e2 e3>>.
+Proof.
+  apply rtc_rtcn in STEPS. des.
+  exploit steps_pf_steps_aux; eauto. i. des.
+  exploit rtcn_rtc; eauto.
+Qed.
